specs/ecdsap256/Spec.P256.fst
@@ -172,12 +172,6 @@ let isPointOnCurve p =
   (x * x * x + aCoordinateP256 * x + bCoordinateP256) % prime
 
 
-let point_prime_to_coordinates (p:point_seq) =
-  felem_seq_as_nat (Lib.Sequence.sub p 0 4),
-  felem_seq_as_nat (Lib.Sequence.sub p 4 4),
-  felem_seq_as_nat (Lib.Sequence.sub p 8 4)
-
-
 val toJacobianCoordinates: tuple2 nat nat -> tuple3 nat nat nat
 let toJacobianCoordinates (r0, r1) = (r0, r1, 1)
 
